Changed logical order of requires and reads clauses on functions.  Reads clauses can now assume the precondition (as had also been the case back in the days when reads clauses had to be self framing).

Source/Dafny/Translator.cs
@@ -4027,18 +4027,21 @@ namespace Microsoft.Dafny {
 
       DefineFrame(f.tok, f.Reads, builder, locals, null);
 
-      // check well-formedness of the preconditions (including termination, and reads checks), and then
-      // assume each one of them
-
-      // check well-formedness of the reads clause
-      var wfo = new WFOptions(null, true, true /* do delayed reads checks over requires */);
-      CheckFrameWellFormed(wfo, f.Reads, locals, builder, etran);
-      wfo.ProcessSavedReadsChecks(locals, builderInitializationArea, builder);
-
-      wfo = new WFOptions(null, true, true /* do delayed reads checks */);
+      // Check well-formedness of the preconditions (including termination), and then
+      // assume each one of them.  After all that (in particular, after assuming all
+      // of them), do the postponed reads checks.
+      var wfo = new WFOptions(null, true, true /* do delayed reads checks */);
       foreach (Expression p in f.Req) {
         CheckWellformedAndAssume(p, wfo, locals, builder, etran);
       }
+      wfo.ProcessSavedReadsChecks(locals, builderInitializationArea, builder);
+
+      // Check well-formedness of the reads clause.  Note that this is done after assuming
+      // the preconditions.  In other words, the well-formedness of the reads clause is
+      // allowed to assume the precondition (yet, the requires clause is checked to
+      // read only those things indicated in the reads clause).
+      wfo = new WFOptions(null, true, true /* do delayed reads checks */);
+      CheckFrameWellFormed(wfo, f.Reads, locals, builder, etran);
       wfo.ProcessSavedReadsChecks(locals, builderInitializationArea, builder);
 
       // check well-formedness of the decreases clauses (including termination, but no reads checks)
